Iterator/Combinators/FilterMap.lean
@@ -24,17 +24,26 @@ section FilterMapMH
 
 universe u' v' u v
 
+@[ext]
 structure FilterMapMH (α : Type u) {β : Type v} (γ : Type v') {γ' : Type w} (γEquiv : Equiv γ γ')
     {m : Type w → Type w'} (f : β → m (Option γ')) where
   inner : α
 
-variable {α : Type w} {α' : Type u} {m : Type w → Type w'} {β : Type v} {γ : Type v'} {γ' : Type w}
-    [Monad m] [Iterator α α' m β]
+variable {α : Type u} {m : Type w → Type w'} {β : Type v} {γ : Type v'} {γ' : Type w}
+    [Monad m] [Iterator α m β]
     {γEquiv : Equiv γ γ'} {f : β → m (Option γ')}
 
-instance [Iterator α α' m β] : SimpleIterator (FilterMapMH α γ γEquiv f) (FilterMapMH α' γ γEquiv f) m γ where
+instance [Iterator α m β] : SimpleIterator (FilterMapMH α γ γEquiv f) m γ where
+  αInternal := FilterMapMH (IterState α m) γ γEquiv f
   βInternal := γ'
-  αEquiv := sorry
+  αEquiv := by
+    refine ⟨fun it => ⟨Iterator.αEquiv.hom it.inner⟩, fun it => ⟨Iterator.αEquiv.inv it.inner⟩, ?_, ?_⟩
+    · intro
+      ext
+      exact Iterator.αEquiv.hom_inv
+    · intro
+      ext
+      exact Iterator.αEquiv.inv_hom
   βEquiv := γEquiv
   step it :=
     matchStep it.inner
@@ -64,8 +73,9 @@ instance [Finite α m] : SimpleIterator.Finite (FilterMapMH α γ γEquiv f) m w
     · cases successor_done.mp h
 
 @[inline]
-def Iterator.filterMapMH [Monad m] [Iterator α α' m β] (f : β → CodensityT m (Option γ)) (γEquiv : Equiv γ γ') (it : α) :
-    FilterMapMH α γ γEquiv (fun b => f b _ (pure <| ·.map γEquiv.hom)) :=
+def Iterator.filterMapMH [Monad m] [Iterator α m β] (f : β → CodensityT m (Option γ)) (γEquiv : Equiv γ γ') (it : IterState α m) :
+    --FilterMapMH (IterState α m) γ γEquiv (fun b => f b _ (pure <| ·.map γEquiv.hom)) :=
+    IterState (FilterMapMH α γ γEquiv (fun b => f b _ (pure <| ·.map γEquiv.hom))) m :=
   ⟨it⟩
 
 /--
@@ -92,7 +102,7 @@ it.filterMapMH     ---a'-----c'-------⊥
 This combinator incurs an additional O(1) cost with each output of `it` in addition to the cost of the monadic effects.
 -/
 @[inline]
-def Iter.filterMapMH [Monad m] [Iterator α α' m β] (f : β → CodensityT m (Option γ)) (γEquiv : Equiv γ γ')
+def Iter.filterMapMH [Monad m] [Iterator α m β] (f : β → CodensityT m (Option γ)) (γEquiv : Equiv γ γ')
     (it : Iter (α := α) m β) :=
   ((toIter m <| Iterator.filterMapMH f γEquiv it.inner) : Iter m γ)
 
@@ -122,7 +132,7 @@ _TODO_: prove `Productive`. This requires us to wrap the FilterMapMH into a new 
 This combinator incurs an additional O(1) cost with each output of `it` in addition to the cost of the monadic effects.
 -/
 @[inline]
-def Iter.mapMH [Monad m] [Iterator α α' m β] (f : β → CodensityT m γ) (γEquiv : Equiv γ γ') (it : Iter (α := α) m β) :=
+def Iter.mapMH [Monad m] [Iterator α m β] (f : β → CodensityT m γ) (γEquiv : Equiv γ γ') (it : Iter (α := α) m β) :=
   (it.filterMapMH (fun b => by exact some <$> f b) γEquiv : Iter m γ)
 
 /--
@@ -149,7 +159,7 @@ it.filterMH        ---a-----c-------⊥
 This combinator incurs an additional O(1) cost with each output of `it` in addition to the cost of the monadic effects.
 -/
 @[inline]
-def Iter.filterMH [Monad m] [Iterator α α' m β] (f : β → CodensityT m Bool) (it : Iter (α := α) m β) :=
+def Iter.filterMH [Monad m] [Iterator α m β] (f : β → CodensityT m Bool) (it : Iter (α := α) m β) :=
   (it.filterMapMH
     (fun b => (f b).mapH (if · then some b else none))
     (Iterator.βEquiv (α := α) (m := m)) : Iter m β)
@@ -160,54 +170,54 @@ section FilterMapH
 
 universe u' v' u v
 
-variable {α : Type w} {α' : Type u} {β : Type v} {m : Type w → Type w'} [Monad m] [Iterator α α' m β]
+variable {α : Type u} {β : Type v} {m : Type w → Type w'} [Monad m] [Iterator α m β]
     {γ : Type v'} {γ' : Type w} {f : β → Option γ}
 
 @[inline]
-def Iter.filterMapH [Monad m] [Iterator α α' m β] (f : β → Option γ) (γEquiv : Equiv γ γ') (it : Iter (α := α) m β) :=
+def Iter.filterMapH [Monad m] [Iterator α m β] (f : β → Option γ) (γEquiv : Equiv γ γ') (it : Iter (α := α) m β) :=
   (it.filterMapMH (pure ∘ f : β → CodensityT m (Option γ)) γEquiv : Iter m γ)
 
 @[inline]
-def Iter.mapH [Monad m] [Iterator α α' m β] (f : β → γ) (γEquiv : Equiv γ γ') (it : Iter (α := α) m β) :=
+def Iter.mapH [Monad m] [Iterator α m β] (f : β → γ) (γEquiv : Equiv γ γ') (it : Iter (α := α) m β) :=
   (it.filterMapH (some ∘ f) γEquiv : Iter m γ)
 
 end FilterMapH
 
 section FilterMap
 
-variable {m : Type w → Type w'} {α : Type w} {α' : Type u} {β : Type v} {γ : Type w} {f : β → Option γ}
+variable {m : Type w → Type w'} {α : Type u} {β : Type v} {γ : Type w} {f : β → Option γ}
 
 -- Potential other formulation of iterators: Each iterator type comes with equivalences for all types of the current level.
 -- Then the following operations could be stated in higher generality, not requiring y : Type w.
 
 @[inline]
-def Iter.filterMap [Iterator α α' m β] [Monad m] (f : β → Option γ) (it : Iter (α := α) m β) :=
+def Iter.filterMap [Iterator α m β] [Monad m] (f : β → Option γ) (it : Iter (α := α) m β) :=
   (it.filterMapH f Equiv.id : Iter m γ)
 
 @[inline]
-def Iter.map [Iterator α α' m β] [Monad m] (f : β → γ) (it : Iter (α := α) m β) :=
+def Iter.map [Iterator α m β] [Monad m] (f : β → γ) (it : Iter (α := α) m β) :=
   (it.filterMap (some ∘ f) : Iter m γ)
 
 @[inline]
-def Iter.filter [Iterator α α' m β] [Monad m] (f : β → Bool) (it : Iter (α := α) m β) :=
+def Iter.filter [Iterator α m β] [Monad m] (f : β → Bool) (it : Iter (α := α) m β) :=
   (it.filterMapH (fun b => if f b then some b else none) (Iterator.βEquiv (α := α) (m := m)) : Iter m β)
 
 end FilterMap
 
 section FilterMapM
 
-variable {m : Type w → Type w} {α : Type w} {α' : Type u} {β : Type v} {γ : Type w} {f : β → Option γ}
+variable {m : Type w → Type w} {α : Type u} {β : Type v} {γ : Type w} {f : β → Option γ}
 
 @[inline]
-def Iter.filterMapM [Iterator α α' m β] [Monad m] (f : β → m (Option γ)) (it : Iter (α := α) m β) :=
+def Iter.filterMapM [Iterator α m β] [Monad m] (f : β → m (Option γ)) (it : Iter (α := α) m β) :=
   (it.filterMapMH (monadLift ∘ f) Equiv.id : Iter m γ)
 
 @[inline]
-def Iter.mapM [Iterator α α' m β] [Monad m] (f : β → m γ) (it : Iter (α := α) m β) :=
+def Iter.mapM [Iterator α m β] [Monad m] (f : β → m γ) (it : Iter (α := α) m β) :=
   (it.filterMapM (fun b => some <$> f b) : Iter m γ)
 
 @[inline]
-def Iter.filterM [Iterator α α' m β] [Monad m] (f : β → m (ULift Bool)) (it : Iter (α := α) m β) :=
+def Iter.filterM [Iterator α m β] [Monad m] (f : β → m (ULift Bool)) (it : Iter (α := α) m β) :=
   (it.filterMapMH
     (fun b => CodensityT.eval (f b) |>.mapH (if ·.down then some b else none))
     (Iterator.βEquiv (α := α) (m := m)) : Iter m β)
