Iterator/MWE.lean
@@ -6,7 +6,7 @@ import Iterator.Combinators.FlatMap
 set_option trace.compiler.ir.result true in
 set_option compiler.small 2 in
 def test (l : List Nat) : Nat :=
-  go (l.iter Id |>.map (· * 2) |>.take 5) 0
+  go (l.iter Id |>.map (· * 2)) 0
 where
   go it acc :=
     match it.step with
@@ -17,14 +17,16 @@ where
 
 set_option pp.universes true in
 set_option pp.explicit true in
-def firstOfEach {α} (l : List (List α)) :=
-  let it := List.iter l Id |>.flatMapS (List.iter · Id)
+set_option trace.compiler.ir.result true in
+set_option compiler.small 10 in
+def firstOfEach (l : List (List Nat)) :=
+  let it := List.iter l Id |>.flatMap (List.iter · Id |>.take 1)
   go (it) 0
 where
   go it acc : Nat :=
     match it.step with
-    | .yield it' x _ => sorry --go it' acc --(acc + x)
-    | .skip it' _ => sorry--go it' acc
+    | .yield it' x _ => go it' (acc)
+    | .skip it' _ => go it' acc
     | .done _ => acc
   termination_by it-- .terminationByFinite
   decreasing_by all_goals sorry
